TSO view: merge into promising
Signed-off-by: Kyeongmin Cho <kyeongmin.cho@kaist.ac.kr>

src/equiv/TsoVtoP.v
@@ -17,126 +17,94 @@ Require Import PromisingArch.lib.Time.
 Require Import PromisingArch.lib.Lang.
 Require Import PromisingArch.promising.CommonPromising.
 Require Import PromisingArch.promising.TsoPromising.
-Require Import PromisingArch.promising.TsoView.
 
 Set Implicit Arguments.
 
 
-Inductive sim_state (vstate:State.t (A:=unit)) (pstate:State.t (A:=unit)): Prop :=
-| sim_state_intro
-    (STMTS: vstate.(State.stmts) = pstate.(State.stmts))
-    (RMAP: vstate.(State.rmap) = pstate.(State.rmap))
-.
-Hint Constructors sim_state.
-
-Inductive sim_local (vlocal:TsoView.Local.t) (plocal:TsoPromising.Local.t): Prop :=
-| sim_local_intro
-    (COH: vlocal.(TsoView.Local.coh) = plocal.(TsoPromising.Local.coh))
-    (VRN: vlocal.(TsoView.Local.vrn) = plocal.(TsoPromising.Local.vrn))
-.
-Hint Constructors sim_local.
-
-Inductive sim_machine (vm:TsoView.Machine.t) (pm:TsoPromising.Machine.t): Prop :=
-| sim_machine_intro
-    (TPOOL: IdMap.Forall2
-              (fun _ vsl psl =>
-                <<STATE: sim_state (fst vsl) (fst psl)>> /\
-                <<LOCAL: sim_local (snd vsl) (snd psl)>>)
-              vm.(TsoView.Machine.tpool) pm.(TsoPromising.Machine.tpool))
-    (MEM: vm.(TsoView.Machine.mem) = pm.(TsoPromising.Machine.mem))
-.
-Hint Constructors sim_machine.
-
 Lemma sim_machine_step
       vm1 vm2 pm1
-      (WF: TsoView.Machine.wf vm1)
-      (STEP: TsoView.Machine.step TsoView.ExecUnit.step vm1 vm2)
-      (SIM: sim_machine vm1 pm1)
-      (NOPROMISE: TsoPromising.Machine.no_promise pm1):
+      (WF: Machine.wf vm1)
+      (VNOPROMISE: Machine.no_promise vm1)
+      (STEP: Machine.step ExecUnit.view_step vm1 vm2)
+      (SIM: Machine.equiv vm1 pm1)
+      (NOPROMISE: Machine.no_promise pm1):
   exists pm2,
-    <<STEP: rtc (TsoPromising.Machine.step TsoPromising.ExecUnit.step) pm1 pm2>> /\
-    <<SIM: sim_machine vm2 pm2>> /\
-    <<NOPROMISE: TsoPromising.Machine.no_promise pm2>>.
+    <<STEP: rtc (Machine.step ExecUnit.step) pm1 pm2>> /\
+    <<SIM: Machine.equiv vm2 pm2>> /\
+    <<NOPROMISE: Machine.no_promise pm2>>.
 Proof.
-  inv SIM. inv STEP. generalize (TPOOL tid). intro TP. inv TP; rewrite FIND in *; ss.
-  inv H0. destruct st1 as [stmts1 rmap1].
-  destruct b as [[pstmts1 prmap1] plc1].
-  symmetry in H. des; ss.
-  inv STATE. ss. subst. rename LOCAL into SIM_LOCAL.
+  inv SIM. inv STEP. rewrite MEM in *.
+  generalize (TPOOL tid). intro TPEQ. rewrite TPEQ in *.
   inv STEP0. inv STEP. inv STATE; inv LOCAL; inv EVENT; ss; subst.
   - (* skip *)
-    eexists (TsoPromising.Machine.mk _ _). esplits.
+    eexists (Machine.mk _ _). esplits.
     + econs; eauto. econs; ss; eauto.
       econs 1. econs. econs; econs; ss.
-    + econs; ss; cycle 1.
-      { rewrite <- MEM. rewrite MEM0. ss. }
+    + econs; ss.
       ii. rewrite TPOOL0. repeat rewrite IdMap.add_spec. repeat condtac; ss.
-      econs. splits; ss.
     + inv NOPROMISE. econs; ss. i.
-      rewrite IdMap.add_spec in *. destruct (tid0 == tid).
-      * apply PROMISES in H. inv FIND0. ss.
-      * eapply PROMISES. eauto.
+      rewrite IdMap.add_spec in *. destruct (tid0 == tid); [inv FIND0|]; eapply PROMISES; eauto.
   - (* assign *)
-    eexists (TsoPromising.Machine.mk _ _). esplits.
+    eexists (Machine.mk _ _). esplits.
     + econs; eauto. econs; ss; eauto.
       econs 1. econs. econs; econs; ss.
-    + econs; ss; cycle 1.
-      { rewrite <- MEM. rewrite MEM0. ss. }
+    + econs; ss.
       ii. rewrite TPOOL0. repeat rewrite IdMap.add_spec. repeat condtac; ss.
-      econs. splits; ss.
     + inv NOPROMISE. econs; ss. i.
-      rewrite IdMap.add_spec in *. destruct (tid0 == tid).
-      * apply PROMISES in H. inv FIND0. ss.
-      * eapply PROMISES. eauto.
+      rewrite IdMap.add_spec in *. destruct (tid0 == tid); [inv FIND0|]; eapply PROMISES; eauto.
   - (* read *)
-    inv SIM_LOCAL. inv STEP. rewrite COH, VRN, MEM in *.
-    eexists (TsoPromising.Machine.mk _ _). esplits.
+    inv STEP.
+    eexists (Machine.mk _ _). esplits.
     + econs; eauto. econs; ss; eauto.
       econs 1. econs. econs; ss.
       { econs; ss. }
       econs 2; ss. econs; try exact LATEST; eauto.
     + econs; ss.
       ii. rewrite TPOOL0. repeat rewrite IdMap.add_spec. repeat condtac; ss.
-      econs. splits; ss.
     + inv NOPROMISE. econs; ss. i.
       rewrite IdMap.add_spec in *. destruct (tid0 == tid).
-      * apply PROMISES in H. inv FIND0. ss.
+      * inv FIND0. apply PROMISES in FIND. ss.
       * eapply PROMISES. eauto.
   - (* write *)
-    inv SIM_LOCAL. inv STEP. rewrite COH, VRN, MEM in *.
+    remember lc2. guardH Heqt.
+    rewrite <- TPEQ in FIND. generalize FIND. intro NPROM.
+    inv VNOPROMISE. eapply PROMISES in NPROM. clear PROMISES.
+    inv STEP.
 
-    assert (PROMISE: exists plc2 mem,
-                      TsoPromising.Local.promise
-                        (ValA.val (sem_expr prmap1 eloc))
-                        (ValA.val (sem_expr prmap1 eval))
-                        ts tid plc1 (TsoPromising.Machine.mem pm1) plc2 mem).
+    assert (PROMISE: exists lcmid mem,
+                      Local.promise
+                        (ValA.val (sem_expr rmap eloc))
+                        (ValA.val (sem_expr rmap eval))
+                        ts tid lc1 (Machine.mem pm1) lcmid mem).
     { esplits. econs; eauto. }
     des.
 
-    assert (FULFILL: exists plc3,
-                      TsoPromising.Local.fulfill
-                        (sem_expr prmap1 eloc)
-                        (sem_expr prmap1 eval)
-                        (ValA.mk _ 0 bot) ts tid plc2 mem plc3).
-    { inv WF. apply WF0 in FIND. inv FIND.
+    assert (FULFILL: Local.fulfill
+                       (sem_expr rmap eloc)
+                       (sem_expr rmap eval)
+                       (ValA.mk _ 0 bot) ts tid lcmid mem lc2).
+    { generalize FIND. intro PWF.
+      inv WF. apply WF0 in PWF. inv PWF.
       inv LOCAL. inv COHMAX. inv COHMAX0; ss. rewrite COH in *.
       inv PROMISE. rewrite MEM0 in MEM2. inv MEM2.
       generalize MEM0. intro X. inv X.
-      esplits. econs; eauto.
+      esplits. econs; eauto; ss.
       - econs; eauto; ss.
         + econs; ss.
         + inv MEM0. rewrite MEM in *.
-          specialize (COH0 mloc). lia.
+          specialize (COH mloc). lia.
       - eapply Memory.append_spec; eauto. ss.
-      - ss. rewrite Promises.set_o. condtac; [|congr]. ss.
+      - rewrite Promises.set_o. condtac; [|congr]. ss.
+      - unguardH Heqt. subst.
+        rewrite NPROM. rewrite Promises.unset_set_bot. ss.
     }
     des.
 
-    eexists (TsoPromising.Machine.mk _ _). esplits.
+    eexists (Machine.mk _ _). esplits.
     + econs 2.
       { (* 1. promise *)
-        econs; ss; eauto.
-        - econs 2. instantiate (1 := TsoPromising.Machine.mk _ mem). econs; eauto; ss.
+        rewrite TPEQ in FIND. econs; ss; eauto.
+        - econs 2. instantiate (1 := Machine.mk _ mem). econs; eauto; ss.
         - ss.
       }
       econs 2; eauto.
@@ -146,54 +114,53 @@ Proof.
         { econs 4; ss. }
         econs 3; eauto.
       * rewrite IdMap.add_spec. condtac; ss. congr.
-    + econs; ss; cycle 1.
+    + rewrite <- Heqt. econs; ss; cycle 1.
       { inv PROMISE. rewrite MEM0 in MEM2. inv MEM2. ss. }
       ii. rewrite TPOOL0. repeat rewrite IdMap.add_spec. repeat condtac; ss.
-      econs. splits; ss.
-      inv PROMISE. inv FULFILL. econs; ss.
     + inv NOPROMISE. econs; ss. i.
       rewrite IdMap.add_spec in *. destruct (tid0 == tid).
-      * apply PROMISES in H. inv FIND0. inv PROMISE. inv FULFILL. ss.
-        rewrite H. funext. i.
-        unfold Promises.unset, Promises.set. destruct (Promises.id_of_time ts); ss.
-        funtac.
+      * inv FIND0. inv PROMISE. inv FULFILL. ss.
+        rewrite NPROM. rewrite Promises.unset_set_bot. ss.
       * rewrite IdMap.add_spec in *. destruct (tid0 == tid); ss. eapply PROMISES. eauto.
   - (* rmw *)
-    inv SIM_LOCAL. inv STEP. rewrite COH, VRN, MEM in *.
+    remember lc2. guardH Heqt.
+    rewrite <- TPEQ in FIND. generalize FIND. intro NPROM.
+    inv VNOPROMISE. eapply PROMISES in NPROM. clear PROMISES.
+    inv STEP.
 
-    assert (PROMISE: exists plc2 mem,
-                      TsoPromising.Local.promise
-                        (ValA.val (sem_expr prmap1 eloc))
+    assert (PROMISE: exists lcmid mem,
+                      Local.promise
+                        (ValA.val (sem_expr rmap eloc))
                         (ValA.val vnew)
-                        ts tid plc1 (TsoPromising.Machine.mem pm1) plc2 mem).
+                        ts tid lc1 (Machine.mem pm1) lcmid mem).
     { esplits. econs; eauto. }
     des.
 
-    assert (PRMW: exists plc3,
-                   TsoPromising.Local.rmw
-                     (sem_expr prmap1 eloc)
-                     vold vnew old_ts ts tid plc2 mem plc3).
-    { inv WF. apply WF0 in FIND. inv FIND.
-      inv LOCAL. inv COHMAX. inv COHMAX0; ss. rewrite COH in *.
+    assert (PRMW: Local.rmw (sem_expr rmap eloc) vold vnew old_ts ts tid lcmid mem lc2).
+    { generalize FIND. intro PWF.
+      inv WF. apply WF0 in PWF. inv PWF.
+      inv LOCAL. inv COHMAX. inv COHMAX0; ss. rewrite COH0 in *.
       inv PROMISE. rewrite MEM0 in MEM2. inv MEM2. inv MEM0.
       esplits. econs; eauto.
       - exploit Memory.read_spec; eauto. lia.
-      - rewrite <- H2 in *. ss.
+      - rewrite <- H1 in *. ss.
       - eapply Memory.read_mon. ss.
       - econs; eauto; ss.
         + econs; ss.
         + rewrite MEM in *.
-          specialize (COH1 mloc). lia.
+          specialize (COH0 mloc). lia.
       - eapply Memory.append_spec; eauto. ss.
       - ss. rewrite Promises.set_o. condtac; [|congr]. ss.
+      - unguardH Heqt. subst.
+        rewrite NPROM. rewrite Promises.unset_set_bot. ss.
     }
     des.
 
-    eexists (TsoPromising.Machine.mk _ _). esplits.
+    eexists (Machine.mk _ _). esplits.
     + econs 2.
       { (* 1. promise *)
-        econs; ss; eauto.
-        - econs 2. instantiate (1 := TsoPromising.Machine.mk _ mem). econs; eauto; ss.
+        rewrite TPEQ in FIND. econs; ss; eauto.
+        - econs 2. instantiate (1 := Machine.mk _ mem). econs; eauto; ss.
         - ss.
       }
       econs 2; eauto.
@@ -203,59 +170,48 @@ Proof.
         { econs 5; eauto. }
         econs 4; eauto.
       * rewrite IdMap.add_spec. condtac; ss. congr.
-    + econs; ss; cycle 1.
+    + rewrite <- Heqt. econs; ss; cycle 1.
       { inv PROMISE. rewrite MEM0 in MEM2. inv MEM2. ss. }
       ii. rewrite TPOOL0. repeat rewrite IdMap.add_spec. repeat condtac; ss.
-      econs. splits; ss.
-      inv PROMISE. inv PRMW. econs; ss.
     + inv NOPROMISE. econs; ss. i.
       rewrite IdMap.add_spec in *. destruct (tid0 == tid).
-      * apply PROMISES in H. inv FIND0. inv PROMISE. inv PRMW. ss.
-        rewrite H. funext. i.
-        unfold Promises.unset, Promises.set. destruct (Promises.id_of_time ts); ss.
-        funtac.
+      * inv FIND0. inv PROMISE. inv PRMW. ss.
+        rewrite NPROM. rewrite Promises.unset_set_bot. ss.
       * rewrite IdMap.add_spec in *. destruct (tid0 == tid); ss. eapply PROMISES. eauto.
   - (* rmw_failure *)
-    inv SIM_LOCAL. inv STEP. rewrite COH, VRN, MEM in *.
-    eexists (TsoPromising.Machine.mk _ _). esplits.
+    inv STEP.
+    eexists (Machine.mk _ _). esplits.
     + econs; eauto. econs; ss; eauto.
       econs 1. econs. econs; ss.
       { inversion RMW. inv H0. econs 6; ss. }
       econs 5; ss. econs; try exact LATEST; eauto.
     + econs; ss.
       ii. rewrite TPOOL0. repeat rewrite IdMap.add_spec. repeat condtac; ss.
-      econs. splits; ss.
     + inv NOPROMISE. econs; ss. i.
       rewrite IdMap.add_spec in *. destruct (tid0 == tid).
-      * apply PROMISES in H. inv FIND0. ss.
+      * inv FIND0. apply PROMISES in FIND. ss.
       * eapply PROMISES. eauto.
   - (* dmb *)
-    inv SIM_LOCAL. inv STEP. rewrite COH, VRN, MEM in *.
-    eexists (TsoPromising.Machine.mk _ _). esplits.
+    inv STEP.
+    eexists (Machine.mk _ _). esplits.
     + econs; eauto. econs; ss; eauto.
       econs 1. econs. econs; ss.
       { econs; ss. }
-      econs 6; ss. econs; eauto.
-      inv COHMAX. rewrite COH in *. econs; eauto.
+      econs 6; ss. econs; try exact LATEST; eauto.
     + econs; ss.
       ii. rewrite TPOOL0. repeat rewrite IdMap.add_spec. repeat condtac; ss.
-      econs. splits; ss.
     + inv NOPROMISE. econs; ss. i.
       rewrite IdMap.add_spec in *. destruct (tid0 == tid).
-      * apply PROMISES in H. inv FIND0. ss.
+      * inv FIND0. apply PROMISES in FIND. ss.
       * eapply PROMISES. eauto.
   - (* dowhile *)
-    eexists (TsoPromising.Machine.mk _ _). esplits.
+    eexists (Machine.mk _ _). esplits.
     + econs; eauto. econs; ss; eauto.
       econs 1; ss. econs. econs; ss; econs; ss.
-    + econs; ss; cycle 1.
-      { rewrite <- MEM. rewrite MEM0. ss. }
+    + econs; ss.
       ii. rewrite TPOOL0. repeat rewrite IdMap.add_spec. repeat condtac; ss.
-      econs. splits; ss.
     + inv NOPROMISE. econs; ss. i.
-      rewrite IdMap.add_spec in *. destruct (tid0 == tid).
-      * apply PROMISES in H. inv FIND0. ss.
-      * eapply PROMISES. eauto.
+      rewrite IdMap.add_spec in *. destruct (tid0 == tid); [inv FIND0|]; eapply PROMISES; eauto.
 
   Grab Existential Variables.
   auto. (* vold when rmw_failure *)
@@ -263,34 +219,35 @@ Qed.
 
 Lemma sim_machine_rtc_step
       vm1 vm2 pm1
-      (WF: TsoView.Machine.wf vm1)
-      (STEP: rtc (TsoView.Machine.step ExecUnit.step) vm1 vm2)
-      (SIM: sim_machine vm1 pm1)
-      (NOPROMISE: TsoPromising.Machine.no_promise pm1):
+      (WF: Machine.wf vm1)
+      (VNOPROMISE: Machine.no_promise vm1)
+      (STEP: rtc (Machine.step ExecUnit.view_step) vm1 vm2)
+      (SIM: Machine.equiv vm1 pm1)
+      (NOPROMISE: Machine.no_promise pm1):
   exists pm2,
-    <<STEP: rtc (TsoPromising.Machine.step TsoPromising.ExecUnit.step) pm1 pm2>> /\
-    <<SIM: sim_machine vm2 pm2>> /\
-    <<NOPROMISE: TsoPromising.Machine.no_promise pm2>>.
+    <<STEP: rtc (Machine.step ExecUnit.step) pm1 pm2>> /\
+    <<SIM: Machine.equiv vm2 pm2>> /\
+    <<NOPROMISE: Machine.no_promise pm2>>.
 Proof.
   revert WF SIM NOPROMISE. revert pm1. induction STEP; eauto. i.
   exploit sim_machine_step; eauto. i. des.
-  exploit Machine.step_step_wf; eauto. intro WF0.
-  exploit IHSTEP; try exact SIM0; ss. i. des.
+  exploit Machine.step_view_step_wf; eauto. intro WF0.
+  exploit IHSTEP; try exact SIM0; ss.
+  { eapply Machine.step_view_step_no_promise; eauto. }
+  i. des.
   esplits; [etrans; eauto | exact SIM1 |]; eauto.
 Qed.
 
-Theorem promising_to_promising_pf
+Theorem view_to_promising
         p vm
-        (EXEC: TsoView.Machine.exec p vm):
+        (EXEC: Machine.view_exec p vm):
   exists pm,
-    <<STEP: TsoPromising.Machine.exec p pm>> /\
-    <<SIM: sim_machine vm pm>>.
+    <<STEP: Machine.exec p pm>> /\
+    <<SIM: Machine.equiv vm pm>>.
 Proof.
   inv EXEC.
   generalize (Machine.init_wf p). intro WF.
   generalize (Machine.init_no_promise p). intro NOPROMISE.
-  exploit sim_machine_rtc_step; eauto; cycle 1.
-  { i. des. esplits; eauto. }
-  econs; ss. ii. repeat rewrite IdMap.map_spec.
-  destruct (IdMap.find id p); ss. econs; ss.
+  exploit sim_machine_rtc_step; eauto; ss. i. des.
+  esplits; eauto.
 Qed.
